theories/AutoSubst/Ast.v
@@ -34,7 +34,11 @@ Inductive term : Type :=
   | tSnd : term -> term
   | tId : term -> term -> term -> term
   | tRefl : term -> term -> term
-  | tIdElim : term -> term -> term -> term -> term -> term -> term.
+  | tIdElim : term -> term -> term -> term -> term -> term -> term
+  | tXi : ell -> term -> term
+  | tXXi : ell -> term -> term -> term
+  | tEval : ell -> term -> term
+  | tBox : ell -> term -> term.
 
 Lemma congr_tSort {s0 : sort} {t0 : sort} (H0 : s0 = t0) :
   tSort s0 = tSort t0.
@@ -241,6 +245,37 @@ exact (eq_trans
          (ap (fun x => tIdElim t0 t1 t2 t3 t4 x) H5)).
 Qed.
 
+Lemma congr_tXi {s0 : ell} {s1 : term} {t0 : ell} {t1 : term} (H0 : s0 = t0)
+  (H1 : s1 = t1) : tXi s0 s1 = tXi t0 t1.
+Proof.
+exact (eq_trans (eq_trans eq_refl (ap (fun x => tXi x s1) H0))
+         (ap (fun x => tXi t0 x) H1)).
+Qed.
+
+Lemma congr_tXXi {s0 : ell} {s1 : term} {s2 : term} {t0 : ell} {t1 : term}
+  {t2 : term} (H0 : s0 = t0) (H1 : s1 = t1) (H2 : s2 = t2) :
+  tXXi s0 s1 s2 = tXXi t0 t1 t2.
+Proof.
+exact (eq_trans
+         (eq_trans (eq_trans eq_refl (ap (fun x => tXXi x s1 s2) H0))
+            (ap (fun x => tXXi t0 x s2) H1))
+         (ap (fun x => tXXi t0 t1 x) H2)).
+Qed.
+
+Lemma congr_tEval {s0 : ell} {s1 : term} {t0 : ell} {t1 : term}
+  (H0 : s0 = t0) (H1 : s1 = t1) : tEval s0 s1 = tEval t0 t1.
+Proof.
+exact (eq_trans (eq_trans eq_refl (ap (fun x => tEval x s1) H0))
+         (ap (fun x => tEval t0 x) H1)).
+Qed.
+
+Lemma congr_tBox {s0 : ell} {s1 : term} {t0 : ell} {t1 : term} (H0 : s0 = t0)
+  (H1 : s1 = t1) : tBox s0 s1 = tBox t0 t1.
+Proof.
+exact (eq_trans (eq_trans eq_refl (ap (fun x => tBox x s1) H0))
+         (ap (fun x => tBox t0 x) H1)).
+Qed.
+
 Lemma upRen_term_term (xi : nat -> nat) : nat -> nat.
 Proof.
 exact (up_ren xi).
@@ -293,6 +328,11 @@ Fixpoint ren_term (xi_term : nat -> nat) (s : term) {struct s} : term :=
       tIdElim (ren_term xi_term s0) (ren_term xi_term s1)
         (ren_term (upRen_term_term (upRen_term_term xi_term)) s2)
         (ren_term xi_term s3) (ren_term xi_term s4) (ren_term xi_term s5)
+  | tXi s0 s1 => tXi s0 (ren_term (upRen_term_term xi_term) s1)
+  | tXXi s0 s1 s2 =>
+      tXXi s0 (ren_term (upRen_term_term xi_term) s1) (ren_term xi_term s2)
+  | tEval s0 s1 => tEval s0 (ren_term xi_term s1)
+  | tBox s0 s1 => tBox s0 (ren_term xi_term s1)
   end.
 
 Lemma up_term_term (sigma : nat -> term) : nat -> term.
@@ -359,6 +399,12 @@ term :=
         (subst_term (up_term_term (up_term_term sigma_term)) s2)
         (subst_term sigma_term s3) (subst_term sigma_term s4)
         (subst_term sigma_term s5)
+  | tXi s0 s1 => tXi s0 (subst_term (up_term_term sigma_term) s1)
+  | tXXi s0 s1 s2 =>
+      tXXi s0 (subst_term (up_term_term sigma_term) s1)
+        (subst_term sigma_term s2)
+  | tEval s0 s1 => tEval s0 (subst_term sigma_term s1)
+  | tBox s0 s1 => tBox s0 (subst_term sigma_term s1)
   end.
 
 Lemma upId_term_term (sigma : nat -> term) (Eq : forall x, sigma x = tRel x)
@@ -447,6 +493,17 @@ subst_term sigma_term s = s :=
         (idSubst_term sigma_term Eq_term s3)
         (idSubst_term sigma_term Eq_term s4)
         (idSubst_term sigma_term Eq_term s5)
+  | tXi s0 s1 =>
+      congr_tXi (eq_refl s0)
+        (idSubst_term (up_term_term sigma_term) (upId_term_term _ Eq_term) s1)
+  | tXXi s0 s1 s2 =>
+      congr_tXXi (eq_refl s0)
+        (idSubst_term (up_term_term sigma_term) (upId_term_term _ Eq_term) s1)
+        (idSubst_term sigma_term Eq_term s2)
+  | tEval s0 s1 =>
+      congr_tEval (eq_refl s0) (idSubst_term sigma_term Eq_term s1)
+  | tBox s0 s1 =>
+      congr_tBox (eq_refl s0) (idSubst_term sigma_term Eq_term s1)
   end.
 
 Lemma upExtRen_term_term (xi : nat -> nat) (zeta : nat -> nat)
@@ -544,6 +601,19 @@ ren_term xi_term s = ren_term zeta_term s :=
         (extRen_term xi_term zeta_term Eq_term s3)
         (extRen_term xi_term zeta_term Eq_term s4)
         (extRen_term xi_term zeta_term Eq_term s5)
+  | tXi s0 s1 =>
+      congr_tXi (eq_refl s0)
+        (extRen_term (upRen_term_term xi_term) (upRen_term_term zeta_term)
+           (upExtRen_term_term _ _ Eq_term) s1)
+  | tXXi s0 s1 s2 =>
+      congr_tXXi (eq_refl s0)
+        (extRen_term (upRen_term_term xi_term) (upRen_term_term zeta_term)
+           (upExtRen_term_term _ _ Eq_term) s1)
+        (extRen_term xi_term zeta_term Eq_term s2)
+  | tEval s0 s1 =>
+      congr_tEval (eq_refl s0) (extRen_term xi_term zeta_term Eq_term s1)
+  | tBox s0 s1 =>
+      congr_tBox (eq_refl s0) (extRen_term xi_term zeta_term Eq_term s1)
   end.
 
 Lemma upExt_term_term (sigma : nat -> term) (tau : nat -> term)
@@ -642,6 +712,19 @@ subst_term sigma_term s = subst_term tau_term s :=
         (ext_term sigma_term tau_term Eq_term s3)
         (ext_term sigma_term tau_term Eq_term s4)
         (ext_term sigma_term tau_term Eq_term s5)
+  | tXi s0 s1 =>
+      congr_tXi (eq_refl s0)
+        (ext_term (up_term_term sigma_term) (up_term_term tau_term)
+           (upExt_term_term _ _ Eq_term) s1)
+  | tXXi s0 s1 s2 =>
+      congr_tXXi (eq_refl s0)
+        (ext_term (up_term_term sigma_term) (up_term_term tau_term)
+           (upExt_term_term _ _ Eq_term) s1)
+        (ext_term sigma_term tau_term Eq_term s2)
+  | tEval s0 s1 =>
+      congr_tEval (eq_refl s0) (ext_term sigma_term tau_term Eq_term s1)
+  | tBox s0 s1 =>
+      congr_tBox (eq_refl s0) (ext_term sigma_term tau_term Eq_term s1)
   end.
 
 Lemma up_ren_ren_term_term (xi : nat -> nat) (zeta : nat -> nat)
@@ -752,6 +835,23 @@ Fixpoint compRenRen_term (xi_term : nat -> nat) (zeta_term : nat -> nat)
         (compRenRen_term xi_term zeta_term rho_term Eq_term s3)
         (compRenRen_term xi_term zeta_term rho_term Eq_term s4)
         (compRenRen_term xi_term zeta_term rho_term Eq_term s5)
+  | tXi s0 s1 =>
+      congr_tXi (eq_refl s0)
+        (compRenRen_term (upRen_term_term xi_term)
+           (upRen_term_term zeta_term) (upRen_term_term rho_term)
+           (up_ren_ren _ _ _ Eq_term) s1)
+  | tXXi s0 s1 s2 =>
+      congr_tXXi (eq_refl s0)
+        (compRenRen_term (upRen_term_term xi_term)
+           (upRen_term_term zeta_term) (upRen_term_term rho_term)
+           (up_ren_ren _ _ _ Eq_term) s1)
+        (compRenRen_term xi_term zeta_term rho_term Eq_term s2)
+  | tEval s0 s1 =>
+      congr_tEval (eq_refl s0)
+        (compRenRen_term xi_term zeta_term rho_term Eq_term s1)
+  | tBox s0 s1 =>
+      congr_tBox (eq_refl s0)
+        (compRenRen_term xi_term zeta_term rho_term Eq_term s1)
   end.
 
 Lemma up_ren_subst_term_term (xi : nat -> nat) (tau : nat -> term)
@@ -870,6 +970,23 @@ subst_term tau_term (ren_term xi_term s) = subst_term theta_term s :=
         (compRenSubst_term xi_term tau_term theta_term Eq_term s3)
         (compRenSubst_term xi_term tau_term theta_term Eq_term s4)
         (compRenSubst_term xi_term tau_term theta_term Eq_term s5)
+  | tXi s0 s1 =>
+      congr_tXi (eq_refl s0)
+        (compRenSubst_term (upRen_term_term xi_term) (up_term_term tau_term)
+           (up_term_term theta_term) (up_ren_subst_term_term _ _ _ Eq_term)
+           s1)
+  | tXXi s0 s1 s2 =>
+      congr_tXXi (eq_refl s0)
+        (compRenSubst_term (upRen_term_term xi_term) (up_term_term tau_term)
+           (up_term_term theta_term) (up_ren_subst_term_term _ _ _ Eq_term)
+           s1)
+        (compRenSubst_term xi_term tau_term theta_term Eq_term s2)
+  | tEval s0 s1 =>
+      congr_tEval (eq_refl s0)
+        (compRenSubst_term xi_term tau_term theta_term Eq_term s1)
+  | tBox s0 s1 =>
+      congr_tBox (eq_refl s0)
+        (compRenSubst_term xi_term tau_term theta_term Eq_term s1)
   end.
 
 Lemma up_subst_ren_term_term (sigma : nat -> term) (zeta_term : nat -> nat)
@@ -1009,6 +1126,23 @@ ren_term zeta_term (subst_term sigma_term s) = subst_term theta_term s :=
         (compSubstRen_term sigma_term zeta_term theta_term Eq_term s3)
         (compSubstRen_term sigma_term zeta_term theta_term Eq_term s4)
         (compSubstRen_term sigma_term zeta_term theta_term Eq_term s5)
+  | tXi s0 s1 =>
+      congr_tXi (eq_refl s0)
+        (compSubstRen_term (up_term_term sigma_term)
+           (upRen_term_term zeta_term) (up_term_term theta_term)
+           (up_subst_ren_term_term _ _ _ Eq_term) s1)
+  | tXXi s0 s1 s2 =>
+      congr_tXXi (eq_refl s0)
+        (compSubstRen_term (up_term_term sigma_term)
+           (upRen_term_term zeta_term) (up_term_term theta_term)
+           (up_subst_ren_term_term _ _ _ Eq_term) s1)
+        (compSubstRen_term sigma_term zeta_term theta_term Eq_term s2)
+  | tEval s0 s1 =>
+      congr_tEval (eq_refl s0)
+        (compSubstRen_term sigma_term zeta_term theta_term Eq_term s1)
+  | tBox s0 s1 =>
+      congr_tBox (eq_refl s0)
+        (compSubstRen_term sigma_term zeta_term theta_term Eq_term s1)
   end.
 
 Lemma up_subst_subst_term_term (sigma : nat -> term) (tau_term : nat -> term)
@@ -1151,6 +1285,23 @@ subst_term tau_term (subst_term sigma_term s) = subst_term theta_term s :=
         (compSubstSubst_term sigma_term tau_term theta_term Eq_term s3)
         (compSubstSubst_term sigma_term tau_term theta_term Eq_term s4)
         (compSubstSubst_term sigma_term tau_term theta_term Eq_term s5)
+  | tXi s0 s1 =>
+      congr_tXi (eq_refl s0)
+        (compSubstSubst_term (up_term_term sigma_term)
+           (up_term_term tau_term) (up_term_term theta_term)
+           (up_subst_subst_term_term _ _ _ Eq_term) s1)
+  | tXXi s0 s1 s2 =>
+      congr_tXXi (eq_refl s0)
+        (compSubstSubst_term (up_term_term sigma_term)
+           (up_term_term tau_term) (up_term_term theta_term)
+           (up_subst_subst_term_term _ _ _ Eq_term) s1)
+        (compSubstSubst_term sigma_term tau_term theta_term Eq_term s2)
+  | tEval s0 s1 =>
+      congr_tEval (eq_refl s0)
+        (compSubstSubst_term sigma_term tau_term theta_term Eq_term s1)
+  | tBox s0 s1 =>
+      congr_tBox (eq_refl s0)
+        (compSubstSubst_term sigma_term tau_term theta_term Eq_term s1)
   end.
 
 Lemma renRen_term (xi_term : nat -> nat) (zeta_term : nat -> nat) (s : term)
@@ -1317,6 +1468,20 @@ Fixpoint rinst_inst_term (xi_term : nat -> nat) (sigma_term : nat -> term)
         (rinst_inst_term xi_term sigma_term Eq_term s3)
         (rinst_inst_term xi_term sigma_term Eq_term s4)
         (rinst_inst_term xi_term sigma_term Eq_term s5)
+  | tXi s0 s1 =>
+      congr_tXi (eq_refl s0)
+        (rinst_inst_term (upRen_term_term xi_term) (up_term_term sigma_term)
+           (rinstInst_up_term_term _ _ Eq_term) s1)
+  | tXXi s0 s1 s2 =>
+      congr_tXXi (eq_refl s0)
+        (rinst_inst_term (upRen_term_term xi_term) (up_term_term sigma_term)
+           (rinstInst_up_term_term _ _ Eq_term) s1)
+        (rinst_inst_term xi_term sigma_term Eq_term s2)
+  | tEval s0 s1 =>
+      congr_tEval (eq_refl s0)
+        (rinst_inst_term xi_term sigma_term Eq_term s1)
+  | tBox s0 s1 =>
+      congr_tBox (eq_refl s0) (rinst_inst_term xi_term sigma_term Eq_term s1)
   end.
 
 Lemma rinstInst'_term (xi_term : nat -> nat) (s : term) :
