theories/Syntax/BasicAst.v
@@ -4,3 +4,32 @@ Inductive sort : Set :=
   | set : sort.
 
 Definition sort_of_product (s s' : sort) := set.
+
+Definition ell_list := list (prod nat bool).
+
+Fixpoint lt_ell n (ℓ : ell_list) : Prop :=
+  match ℓ with
+  | nil => True
+  | cons (n', b') ℓ => n < n' /\ (lt_ell n ℓ) 
+  end.
+
+Fixpoint ell_wf (ℓ : ell_list) : Prop :=
+  match ℓ with
+  | nil => True
+  | cons (n, b) ℓ => (lt_ell n ℓ) /\ ell_wf ℓ
+  end.
+
+Inductive SFalse : SProp := .
+Inductive STrue : SProp := SI.
+#[projections(primitive)]Record SAnd (A B : SProp) : SProp := Sconj { Spr1 : A;  Spr2 : B }.
+Arguments Spr1 {A B}.
+Arguments Spr2 {A B}.
+
+
+Definition Sis_true (b : bool) : SProp := if b then STrue else SFalse.
+From Stdlib Require Import Logic.StrictProp.
+
+#[projections(primitive)]Record ell : Set := {
+   ℓ_list :> ell_list;
+   ℓ_wf : Squash (ell_wf ℓ_list);
+   }.
